Fixups for [derived_to_base].

theories/lang/cpp/logic/dispatch.v
@@ -16,14 +16,32 @@ Require Import bedrock.lang.cpp.heap_notations.
 Section with_cpp.
   Context `{Σ : cpp_logic}.
 
-  (* the [offset] to cast a [base] to a [derived] *)
-  Fixpoint base_to_derived {σ : genv} (base : globname) (path : list globname) : offset :=
+  (** [base_to_derived derived path] is the offset to [derived]
+      from the path [path]. For example,
+      [[
+      Eval simpl in base_to_derived "::D" ["::B";"::A";"::X"]%bs.
+      (* = o_id ,, o_derived σ "::X" "::A" ,, o_derived σ "::A" "::B" ,, o_derived σ "::B" "::D" *)
+      ]]
+
+      NOTE the arguments are the same as [derived_to_base] but the direction
+           of the cast is swapped.
+   *)
+  Fixpoint base_to_derived {σ : genv} (derived : globname) (path : list globname) : offset :=
     match path with
     | nil => o_id
-    | derived :: rest => o_dot (o_derived σ base derived) (base_to_derived derived rest)
+    | base :: rest => o_dot (base_to_derived base rest) (o_derived σ base derived)
     end.
 
-  (* the [offset] to cast a [derived] to a [base] *)
+  (** [derived_to_base derived path] is the offset from [derived]
+      from the path [path]. For example,
+      [[
+      Eval simpl in derived_to_base "::D" ["::B";"::A";"::X"]%bs.
+      (* =  o_base σ "::D" "::B" ,, (o_base σ "::B" "::A" ,, (o_base σ "::A" "::X" ,, o_id)) *)
+      ]]
+
+      NOTE the arguments are the same as [base_to_derived] but the direction
+           of the cast is swapped.
+   *)
   Fixpoint derived_to_base {σ : genv} (derived : globname) (path : list globname) : offset :=
     match path with
     | nil => o_id
@@ -33,50 +51,42 @@ Section with_cpp.
   (** If successful, returns a pair of the function pointer to the
    *  implementation and the downcast for [this] pointer. *)
   Definition get_impl {σ} (base : globname) (path : list globname) (f : obj_name)
-    : option (ptr * offset) :=
+    : option (ptr * globname * offset) :=
     match dispatch.dispatch σ base path f with
     | None => None
-    | Some (path, fptr) => Some (_global fptr, base_to_derived base path)
+    | Some (path, cls, fptr) => Some (_global fptr, cls, base_to_derived base path)
     end.
 
   (** [resolve_virtual σ this cls f Q] returns [Q fa this'] if resolving [f] on
-   * [this] results in a function that is equivalent to calling the pointer [fa]
-   * passing [this'] as the "this" argument.
+      [this] results in a function that is equivalent to calling the pointer [fa]
+      passing [this'] as the "this" argument.
    *)
   Definition resolve_virtual {σ : genv}
              (this : ptr) (cls : globname) (f : obj_name)
-             (Q : forall (faddr : ptr) (cls_type : globname) (this_addr : ptr), mpred) : mpred :=
-    Exists σ' mdc (path : list globname),
-      [| class_derives cls path |] **
-        (* ^ we quantify over another program environment because class
-             extension is open, the caller does not need to know the target
-             function.
-           - the [class_derives] fact *must* be in [σ'] because [mdc] might
-             not exist in [σ].
-         *)
-    (<absorb> Exists q, this |-> identityR (σ:=σ') cls path q) //\\
-              (* ^ the [class_compatible σ σ' cls] ensures that the virtual
-                   tables the [cls] class are compatible between the (possibly
-                   different) translation units.
-               *)
+             (Q : forall (faddr : ptr) (cls_type : globname) (this_addr : ptr), mpred)
+    : mpred :=
+    Exists (path : list globname),
+      (Exists q, this |-> identityR (σ:=σ) cls path q ** [| path <> nil |] ** True) //\\
       match get_impl cls path f with
-      | Some (fa, off) => Q fa mdc (_offset_ptr this off)
-      | None => (* the function wasn't found or the implementation was pure virtual *)
+      | Some (fa, cls, off) => Q fa cls (_offset_ptr this off)
+      | None => (* the function was not found or the implementation was pure virtual *)
         False
       end.
 
-  Lemma resolve_virtual_frame:
-    ∀ {σ : genv} (cls : globname) (this : ptr) (Q Q' : ptr → globname → ptr → mpredI) (s : Struct),
-      Forall (a : ptr) (b : globname) (c : ptr), Q a b c -* Q' a b c
-      |-- resolve_virtual this cls (s_dtor s) Q -* resolve_virtual this cls (s_dtor s) Q'.
+  Lemma resolve_virtual_frame {σ : genv} (cls : globname) (this : ptr) s
+    (Q Q' : ptr → globname → ptr → mpredI) :
+        Forall (a : ptr) (b : globname) (c : ptr), Q a b c -* Q' a b c
+    |-- resolve_virtual this cls (s_dtor s) Q -* resolve_virtual this cls (s_dtor s) Q'.
   Proof.
     intros.
     rewrite /resolve_virtual.
-    iIntros "X". iDestruct 1 as (a b c) "Y"; iExists a, b, c.
+    iIntros "X Y".
+    iDestruct "Y" as (path) "Y".
+    iExists path.
     iSplit.
     { iDestruct "Y" as "[$ _]". }
     { iDestruct "Y" as "[_ Y]". case_match => //.
-      destruct p. by iApply "X". }
+      destruct p as [[??]?]. by iApply "X". }
   Qed.
 
 End with_cpp.
