theories/lang/cpp/semantics/dispatch.v
@@ -19,20 +19,10 @@ Require Import bedrock.lang.cpp.semantics.subtyping.
     A* a = new B();
     a->foo(); // same as [static_cast<B*>(a)->B::foo()]
     ```
-    note that in order to dispatch to the overridden function
-    the dispatch also introduces a cast to get a pointer
-    of the correct type.
+    NOTE in order to dispatch to the overridden function
+         the [dispatch] function also introduces a cast to
+         get a pointer of the correct type.
  *)
-Record vhandle : Set :=
-  { (* the name of the method that implements the function
-       [None] means that there is no body.
-     *)
-    vimpl      : option obj_name
-  ; vpath      : list globname
-(*   ; voverrider : globname
-  ; vfrom      : globname
-  ; (* the cast for the [this] parameter *)
-    derivation : class_derives σ voverrider vfrom  *) }.
 
 Section dispatch.
   Context (σ : genv).
@@ -40,10 +30,10 @@ Section dispatch.
   Definition list_get {T} (t : obj_name) (l : list (obj_name * T)) : option T :=
     snd <$> List.find (fun '(t',_) => bool_decide (t = t')) l.
 
-  (** [dispatch base path fn = Some (impl_path, impl_fn)]
+  (** [dispatch path fn = Some (impl_path, impl_fn)]
       dispatches [fn] (the name of a member function on [Tnamed base])
       given the path [path] (which is [mdc..base].
-      NOTE: [base] and [path] are the arguments to [identity]
+      NOTE: [path] takes the form of the [path] argument to [identity].
       - [impl_fn] is the name of the function to call
       - [impl_path] is the path from (base..impl].
       Some examples assuming:
@@ -52,20 +42,21 @@ Section dispatch.
       struct B : public A { virtual void f(); };
       struct C : public B { };
       ```
-      - [dispatch "::A" ["::C","::B","::A"] "A::f()" = Some (["::B"], "B::f()")]
-      - [dispatch "::B" ["::C","::A"] "B::f()" = Some ([], "B::f()")]
+      - [dispatch ["::C","::B","::A"] "A::f()" = Some (["::B"], "B::f()")]
+      - [dispatch ["::C","::A"] "B::f()" = Some ([], "B::f()")]
    *)
   #[local] Fixpoint dispatch (base : globname) (path : list globname) (fn : obj_name)
-    : option (list globname * obj_name) :=
+    : option (list globname * globname * obj_name) :=
     match path with
-    | nil => Some (path, fn)
+    | nil => Some (path, base, fn)
     | next :: rest =>
-        dispatch base rest fn ≫= fun '(hndl, override) =>
+        dispatch base rest fn ≫= fun rr =>
           match σ.(genv_tu) !! next with
           | Some (Gstruct st) =>
+              let '(_, override, _) := rr in
               match list_get override st.(s_overrides) with
-              | Some cand' => Some (path, cand')
-              | None => Some (hndl, override)
+              | Some cand' => Some (path, base, cand')
+              | None => Some rr
               end
           | _ => None
           end
